fixed all the issues with tactics for automatically solving goals

Tactics.v
@@ -1,251 +1,166 @@
 Require Import Lib.EclecticLib Syntax Properties.
 
+Ltac discharge_string_dec := destruct_string_dec; discharge_append.
+
 Ltac discharge_NoSelfCall :=
   unfold NoSelfCallBaseModule, NoSelfCallRulesBaseModule, NoSelfCallMethsBaseModule; split; auto; simpl; intros;
   repeat match goal with
-         | H: _ \/ _ |- _ => destruct H; subst; simpl in *
+         | H: _ \/ _ |- _ => destruct H; subst
          | H: False |- _ => exfalso; apply H
          | |- NoCallActionT _ (convertLetExprSyntax_ActionT _) => apply LetExprNoCallActionT
          | _ => constructor; auto; simpl; try intro; discharge_DisjKey
          end.
 
-Ltac discharge_simulationGeneral mySimRel disjReg :=
-  apply simulationGeneral with (simRel := mySimRel); auto; simpl; intros;
-  (repeat match goal with
-          | H: _ \/ _ |- _ => destruct H
-          | H: False |- _ => exfalso; apply H
-          | H: (?a, ?b) = (?c, ?d) |- _ =>
-            let H2 := fresh in
-            inversion H;
-            pose proof (f_equal snd H) as H2;
-            simpl in H2; subst; clear H; EqDep_subst
-         | H: SemAction _ (convertLetExprSyntax_ActionT ?e) _ _ _ _ |- _ =>
-           apply convertLetExprSyntax_ActionT_full in H; dest; subst
-          | H: SemAction _ _ _ _ _ _ |- _ =>
-            apply inversionSemAction in H; dest; subst
-          | H: if ?P then _ else _ |- _ => case_eq P; let i := fresh in intros i; rewrite ?i in *; dest
-          | H: Forall2 _ _ _ |- _ => inv H
-          | |- exists k, In k _ /\ In k _ =>
-            exists disjReg; rewrite ?map_app, ?in_app_iff; simpl; tauto
-          | H: ?a = ?a |- _ => clear H
-          | H: match convertLetExprSyntax_ActionT ?P with
-               | _ => _
-               end |- _ =>
-            case_eq P; intros;
-            match goal with
-            | H': P = _ |- _ => rewrite ?H' in *; simpl in *; try discriminate
-            end
-          end); dest; simpl in *; repeat subst; simpl in *.
+Ltac discharge_SemAction :=
+  repeat match goal with
+         | |- SemAction _ (If ?p then _ else _ as _; _)%kami_action _ _ _ _ => eapply SemAction_if
+         | |- if ?P then SemAction _ _ _ _ _ _ else SemAction _ _ _ _ _ _ =>
+           case_eq P; let H := fresh in intros H; rewrite ?H in *; try discriminate
+         | |- SemAction _ (convertLetExprSyntax_ActionT _) _ _ _ _ => eapply convertLetExprSyntax_ActionT_same
+         | |- SemAction _ _ _ _ _ _ => econstructor
+         end;
+  rewrite ?key_not_In_fst; unfold not; simpl; try tauto; simpl; intros; discharge_DisjKey.
+
+
+
+
+
+
+
+
+Local Ltac discharge_init :=
+  repeat econstructor;
+  try match goal with
+      | |- match ?P in _ = Y return _ with
+           | eq_refl => _
+           end = _ => is_evar P; match type of P with
+                                 | ?tp = _ => unify P (@eq_refl _ tp)
+                                 end
+      end; simpl; eauto.
 
 Ltac clean_hyp :=
   simpl in *;
   repeat match goal with
-         | H: DisjKey _ _ |- _ => apply DisjKeyWeak_same in H; [unfold DisjKeyWeak in H; simpl in H| apply string_dec]
-         (* | H: In ?x ?ls |- _ => *)
-         (*   apply (InFilterPair string_dec) in H; simpl in H; destruct H; [|exfalso; auto] *)
+         | |- NoSelfCallBaseModule _ => discharge_NoSelfCall
+         | H: DisjKey _ _ |- _ => clear H
+         | H: key_not_In _ _ |- _ => clear H
+         | H: ?a = ?a |- _ => clear H
+         | H: ?a <> ?b |- _ => clear H
+         | H: False |- _ => exfalso; apply H
+         | H: ?a <> ?a |- _ => exfalso; apply (H eq_refl)
          | H: _ \/ _ |- _ => destruct H; subst
-         | H: False |- _ => exfalso; apply H
+         | H: _ /\ _ |- _ => destruct H; subst
+         | H: exists x, _ |- _ => destruct H
          | H: (?A, ?B) = (?P, ?Q) |- _ =>
-           let H1 := fresh in
-           let H2 := fresh in
-           pose proof (f_equal fst H) as H1;
-           pose proof (f_equal snd H) as H2;
-           simpl in H1, H2;
-           clear H
-         | H: ?A = ?A |- _ => clear H
-         | H: (?a ++ ?b)%string = (?a ++ ?c)%string |- _ => rewrite append_remove_prefix in H; subst
-         | H: (?a ++ ?b)%string = (?c ++ ?b)%string |- _ => rewrite append_remove_suffix in H; subst
+           apply inversionPair in H; destruct H as [? ?]; subst
          | H: existT ?a ?b ?c1 = existT ?a ?b ?c2 |- _ => apply Eqdep.EqdepTheory.inj_pair2 in H; subst
-         | H: ?A = ?B |- _ => discriminate
+         | H: existT ?a ?b1 ?c1 = existT ?a ?b2 ?c2 |- _ => apply inversionExistT in H;
+                                                            destruct H as [? ?]; subst
+         | H: (?a ++ ?b)%string = (?a ++ ?c)%string |- _ =>
+           apply append_remove_prefix in H; subst
+         | H: ?a = ?b |- _ => discriminate
          | H: SemAction _ (convertLetExprSyntax_ActionT ?e) _ _ _ _ |- _ =>
-           apply convertLetExprSyntax_ActionT_full in H; dest; subst
+           apply convertLetExprSyntax_ActionT_full in H
+         | H: SemAction _ _ _ _ _ _ |- _ =>
+           apply inversionSemAction in H
+         | H: if ?P then _ else _ |- _ => case_eq P; let i := fresh in intros i; rewrite ?i in *
+         | H: Forall2 _ _ _ |- _ => inv H; dest
+         | H: RegT |- _ => destruct H as [? [? ?]];
+                           repeat (unfold fst, snd, projT1, projT2 in *; subst)
+         | H: In _ _ |- _ => simpl in H
+         | |- exists rspec : list RegT,
+             Forall2 _ _ _ /\ _ _ _ => discharge_init
          end.
 
-Ltac discharge_string_dec :=
-  repeat match goal with
-         | |- context[string_dec ?P ?Q] => destruct (string_dec P Q);
-                                           discharge_appendage;
-                                           try (tauto || congruence)
-         end.
+Ltac discharge_CommonRegister disjReg :=
+  match goal with
+  | |- exists k: string, _ /\ _ =>
+    exists disjReg; simpl; auto; tauto
+  | _ => idtac
+  end.
 
-Ltac discharge_SemAction :=
-  repeat match goal with
-         | |- SemAction _ (If ?p then _ else _ as _; _)%kami_action _ _ _ _ => eapply SemAction_if
-         | |- if ?P then SemAction _ _ _ _ _ _ else SemAction _ _ _ _ _ _ => case_eq P; let H := fresh in intros H; rewrite ?H in *; try discriminate
-         | |- SemAction _ (convertLetExprSyntax_ActionT _) _ _ _ _ => eapply convertLetExprSyntax_ActionT_same
-         | |- SemAction _ _ _ _ _ _ => econstructor
-         end; rewrite ?key_not_In_fst in *; simpl in *; try tauto; simpl in *; unfold not; intros; rewrite ?DisjKeyWeak_same by apply string_dec;
-  unfold DisjKeyWeak; intros; simpl in *;
-  repeat match goal with
-         | H: _ \/ _ |- _ => destruct H; discharge_appendage
-         | H: False |- _ => exfalso; apply H
-         | H: ?a = ?b |- _ => match type of a with
-                              | string => try discriminate
-                              end
-         end.
+Ltac discharge_CommonRegisterAuto :=
+  match goal with
+  | |- exists k: string, _ /\ _ =>
+    eexists; simpl; eauto; tauto
+  | _ => idtac
+  end.
 
-(* Ltac discharge_SemAction := *)
-(*   (repeat match goal with                              *)
-(*           | H: SemAction _ (convertLetExprSyntax_ActionT ?e) _ _ _ _ |- _ => *)
-(*             apply convertLetExprSyntax_ActionT_full in H; dest; subst *)
-(*           | H: SemAction _ _ _ _ _ _ |- _ => *)
-(*             apply inversionSemAction in H; dest; subst *)
-(*           | H: if ?P then _ else _ |- _ => case_eq P; let i := fresh in intros i; rewrite ?i in *; dest *)
-(*           | H: key_not_In _ _ |- _ => clear H *)
-(*           | H: DisjKey _ _ |- _ => clear H *)
-(*           end); *)
-(*   repeat match goal with *)
-(*          | H: In (?a, _) ?ls |- _ => *)
-(*            let HF := fresh in *)
-(*            rewrite (InFilterPair string_dec) in H; simpl in H; discharge_append; *)
-(*            apply InSingleton_impl in H; subst *)
-(*          | H: ?a = ?a |- _ => clear H *)
-(*          | H: ?a <> ?a |- _ => exfalso; apply (H eq_refl) *)
-(*          | H: (_, existT _ _ _) = (_, existT _ _ _) |- _ => *)
-(*            apply inversionExistT in H; destruct H as [? ?] *)
-(*          | H: existT ?a ?b ?c1 = existT ?a ?b ?c2 |- _ => apply Eqdep.EqdepTheory.inj_pair2 in H; subst *)
-(*          | H: ?a <> ?b |- _ => clear H *)
-(*          end. *)
-
-(* Local Ltac clean_hyp := *)
-(*   repeat match goal with *)
-(*          | H: @key_not_In _ _ _ _ |- _ => clear H *)
-(*          end; *)
-(*   repeat match goal with *)
-(*          | H: DisjKey _ _ |- _ => apply DisjKeyWeak_same in H; [unfold DisjKeyWeak in H; simpl in H| apply string_dec] *)
-(*          | H: In ?x ?ls |- _ => *)
-(*            apply (InFilterPair string_dec) in H; simpl in H; destruct H; [|exfalso; auto] *)
-(*          | H: False |- _ => exfalso; apply H *)
-(*          | H: (?A, ?B) = (?P, ?Q) |- _ => *)
-(*            let H1 := fresh in *)
-(*            let H2 := fresh in *)
-(*            pose proof (f_equal fst H) as H1; *)
-(*            pose proof (f_equal snd H) as H2; *)
-(*            simpl in H1, H2; *)
-(*            clear H *)
-(*          | H: ?A = ?A |- _ => clear H *)
-(*          | H: (?a ++ ?b)%string = (?a ++ ?c)%string |- _ => rewrite append_remove_prefix in H; subst *)
-(*          | H: (?a ++ ?b)%string = (?c ++ ?b)%string |- _ => rewrite append_remove_suffix in H; subst *)
-(*          | H: existT ?a ?b ?c1 = existT ?a ?b ?c2 |- _ => apply Eqdep.EqdepTheory.inj_pair2 in H; subst *)
-(*          | H: ?A = ?B |- _ => discriminate *)
-(*          | H: SemAction _ (convertLetExprSyntax_ActionT ?e) _ _ _ _ |- _ => *)
-(*            apply convertLetExprSyntax_ActionT_full in H; dest; subst *)
-(*          end. *)
-
-(* Local Ltac destruct_RegT := *)
-(*   repeat match goal with *)
-(*          | H: RegT |- _ => *)
-(*            destruct H as [? [? ?]]; simpl in *; repeat subst; simpl in * *)
-(*          end. *)
-
-(* Local Ltac discharge_init := *)
-(*   repeat econstructor; eauto; simpl; *)
-(*   instantiate (1 := eq_refl); simpl; auto. *)
-
-(* Local Ltac simplify_Ins := *)
-(*   repeat match goal with *)
-(*          | H: In _ (getRules _) |- _ => simpl in H *)
-(*          | H: In _ (getMethods _) |- _ => simpl in H *)
-(*          | H: _ \/ _ |- _ => destruct H *)
-(*          | H: False |- _ => exfalso; apply H *)
-(*          | H: (_, _) = (_, _) |- _ => inv H *)
-(*          | H: (_, _) = ?a |- _ => try subst a *)
-(*          end. *)
-
-(* Ltac discharge_NoSelfCall := *)
-(*   unfold NoSelfCallBaseModule, NoSelfCallRulesBaseModule, NoSelfCallMethsBaseModule; split; auto; intros; *)
-(*   simplify_Ins; *)
-(*   repeat match goal with *)
-(*          | |- NoCallActionT _ (convertLetExprSyntax_ActionT _) => apply LetExprNoCallActionT *)
-(*          | _ => constructor; auto; cbn - [In]; try rewrite (InFilter string_dec); simpl; unfold getBool, not; intros; *)
-(*                 try (rewrite (DisjKey_filter string_dec)); discharge_append *)
-(*          end. *)
-(*   (* unfold NoSelfCallBaseModule, NoSelfCallRulesBaseModule, NoSelfCallMethsBaseModule; split; auto; intros; *) *)
-(*   (* simplify_Ins; *) *)
-(*   (* repeat match goal with *) *)
-(*   (*        | |- NoCallActionT _ (convertLetExprSyntax_ActionT _) => apply LetExprNoCallActionT *) *)
-(*   (*        | _ => constructor; auto; simpl; try intro; try (rewrite (DisjKey_filter string_dec); discharge_append) *) *)
-(*   (*        end. *) *)
+Ltac discharge_simulationGeneral mySimRel :=
+  apply simulationGeneral with (simRel := mySimRel); auto; simpl; intros;
+  try match goal with
+      | H: mySimRel _ _ |- _ => inv H
+      end;
+  clean_hyp; auto; clean_hyp.
 
 
 
-(* Ltac discharge_simulation myRel := *)
-(*   apply simulationGeneral with (simRel := myRel); intros; auto; *)
-(*   repeat match goal with *)
-(*          | H: Forall2 _ _ _ |- _ => inv H; dest *)
-(*          | H: RegT |- _ => destruct H as [? [? ?]]; *)
-(*                            repeat (unfold fst, snd, projT1, projT2 in *; subst) *)
-(*          | _ => discharge_init *)
-(*          | H: myRel _ _ |- _ => inv H; auto *)
-(*          end; [discharge_NoSelfCall | simplify_Ins; discharge_SemAction | simplify_Ins; discharge_SemAction | simplify_Ins | simplify_Ins]. *)
+Notation sz := 5.
 
+Section Named.
+  Variable name: string.
+  Local Notation "^ x" := (name ++ "." ++ x)%string (at level 0).
 
-(* Notation sz := 5. *)
-
-(* Section Named. *)
-(*   Variable name: string. *)
-(*   Local Notation "^ x" := (name ++ "." ++ x)%string (at level 0). *)
-
-(*     Definition IncrementerImpl := *)
-(*       MODULE_WF { *)
-(*           Register ^"counter" : Bit sz <- Default *)
-(*             with Register ^"counter1" : Bit sz <- Default *)
-(*             with Register ^"isSending" : Bool <- true *)
+    Definition IncrementerImpl :=
+      MODULE_WF {
+          Register ^"counter" : Bit sz <- Default
+            with Register ^"counter1" : Bit sz <- Default
+            with Register ^"isSending" : Bool <- true
                                              
-(*             with Rule ^"send" := *)
-(*             ( Read isSending: Bool <- ^"isSending" ; *)
-(*                 Assert #isSending ; *)
-(*                 Read counter: Bit sz <- ^"counter" ; *)
-(*                 Call "counterVal"(#counter: _); *)
-(*                 Write ^"isSending" <- !#isSending ; *)
-(*                 Retv ) *)
+            with Rule ^"send" :=
+            ( Read isSending: Bool <- ^"isSending" ;
+                Assert #isSending ;
+                Read counter: Bit sz <- ^"counter" ;
+                Call "counterVal"(#counter: _);
+                Write ^"isSending" <- !#isSending ;
+                Retv )
 
-(*             with Rule ^"inc" := *)
-(*               ( Read isSending: Bool <- ^"isSending" ; *)
-(*                   Assert !#isSending ; *)
-(*                   Read counter: Bit sz <- ^"counter" ; *)
-(*                   Write ^"counter" <- #counter + $1; *)
-(*                   Write ^"isSending" <- !#isSending ; *)
-(*                   Retv ) *)
-(*         }. *)
+            with Rule ^"inc" :=
+              ( Read isSending: Bool <- ^"isSending" ;
+                  Assert !#isSending ;
+                  Read counter: Bit sz <- ^"counter" ;
+                  Write ^"counter" <- #counter + $1;
+                  Write ^"isSending" <- !#isSending ;
+                  Retv )
+        }.
 
-(*   Definition IncrementerSpec := *)
-(*     MODULE_WF { *)
-(*         Register ^"counter" : Bit sz <- Default *)
-(*           with Register ^"counter1" : Bit sz <- Default *)
+  Definition IncrementerSpec :=
+    MODULE_WF {
+        Register ^"counter" : Bit sz <- Default
+          with Register ^"counter1" : Bit sz <- Default
                                          
-(*           with Rule ^"send_and_inc" := *)
-(*           ( Read counter: Bit sz <- ^"counter" ; *)
-(*               Call "counterVal"(#counter: _); *)
-(*               Write ^"counter" <- #counter + $1; *)
-(*               Retv) *)
-(*       }. *)
+          with Rule ^"send_and_inc" :=
+          ( Read counter: Bit sz <- ^"counter" ;
+              Call "counterVal"(#counter: _);
+              Write ^"counter" <- #counter + $1;
+              Retv)
+      }.
 
-(*   Record Incrementer_invariant (impl spec: RegsT) : Prop := *)
-(*     { counterImpl: word sz ; *)
-(*       isSending: bool ; *)
-(*       implEq : impl = (^"counter", existT _ (SyntaxKind (Bit sz)) counterImpl) *)
-(*                         :: (^"counter1", existT _ (SyntaxKind (Bit sz)) $0) *)
-(*                         :: (^"isSending", existT _ (SyntaxKind Bool) isSending) :: nil ; *)
-(*       specEq : spec = (^"counter", existT _ (SyntaxKind (Bit sz)) *)
-(*                                          (if isSending then counterImpl else counterImpl ^+ $1)) *)
-(*                         :: (^"counter1", existT  _ (SyntaxKind (Bit sz)) $0) *)
-(*                         :: nil *)
-(*     }. *)
-(* End Named. *)
+  Record Incrementer_invariant (impl spec: RegsT) : Prop :=
+    { counterImpl: word sz ;
+      isSending: bool ;
+      implEq : impl = (^"counter", existT _ (SyntaxKind (Bit sz)) counterImpl)
+                        :: (^"counter1", existT _ (SyntaxKind (Bit sz)) $0)
+                        :: (^"isSending", existT _ (SyntaxKind Bool) isSending) :: nil ;
+      specEq : spec = (^"counter", existT _ (SyntaxKind (Bit sz))
+                                         (if isSending then counterImpl else counterImpl ^+ $1))
+                        :: (^"counter1", existT  _ (SyntaxKind (Bit sz)) $0)
+                        :: nil
+    }.
+End Named.
 
-(* Theorem Incrementer_TraceInclusion (name: string) : *)
-(*   TraceInclusion (Base (IncrementerImpl name)) (Base (IncrementerSpec name)). *)
-(* Proof. *)
-(*   discharge_simulation (Incrementer_invariant name). *)
-(*   - right; do 2 (do 2 eexists; repeat split; eauto; simpl in * ). *)
-(*     * repeat (econstructor; eauto; simpl; subst). *)
-(*       unfold key_not_In; unfold not; intros; simpl in *; auto. *)
-(*     * repeat (econstructor; eauto; simpl; subst). *)
-(*       discharge_append. *)
-(*       rewrite wzero_wplus; auto. *)
-(*   - left; split; auto; simpl in *. *)
-(*     repeat (econstructor; eauto; simpl; subst). *)
-(*     rewrite negb_true_iff in *; subst. *)
-(*     rewrite wzero_wplus; simpl; auto. *)
-(* Qed. *)
+Theorem Incrementer_TraceInclusion (name: string) :
+  TraceInclusion (Base (IncrementerImpl name)) (Base (IncrementerSpec name)).
+Proof.
+  discharge_simulationGeneral (Incrementer_invariant name); discharge_CommonRegisterAuto.
+  - right; do 2 (do 2 eexists; repeat split; eauto; simpl in * ).
+    + discharge_SemAction; subst; auto.
+    + repeat discharge_string_dec.
+      repeat (econstructor; eauto; simpl; subst).
+      rewrite wzero_wplus; auto.
+  - left; split; auto; simpl in *.
+    discharge_string_dec.
+    repeat (econstructor; eauto; simpl; subst).
+    rewrite negb_true_iff in *; subst.
+    rewrite wzero_wplus; simpl; auto.
+Qed.
